toAndFrom DTerm

templateCoqMisc.v
@@ -25,9 +25,11 @@ match n with
 | nAnon => nAnon
 end.
 
+
 Fixpoint mapDbIndices (f:nat -> nat) (t:term) : term :=
 match t with
 | tRel n => tRel (f n)
+
 | _ => (* mapDbIndices f t *) t
 end.
 
@@ -43,3 +45,72 @@ Definition printTerm (name  : ident): TemplateMonad unit :=
   (tmBind (tmQuote name true) tmPrint).
 
 
+Inductive CoqOpid : Set :=
+ | CLambda
+ | CProd
+ | CSort (s: sort)
+ | CCast
+ | CConst
+(* | TFix (nMut index: nat) *)
+(* | NDCon (dc : inductive*nat) (nargs : nat) *)
+ | CApply (nargs:nat)
+(* | NLet *)
+(* | NMatch (dconAndNumArgs : list (dcon * nat)). *)
+ | CUnknown.
+
+Require Import SquiggleEq.termsDB.
+Require Import SquiggleEq.list.
+Import ListNotations.
+Require Import NArith.
+Require Import Program.
+
+Fixpoint toSquiggle (t: term) : (@DTerm Ast.name CoqOpid):=
+match t with
+| tRel n => vterm (N.of_nat n)
+| tSort s => oterm (CSort s) []
+| tLambda n T b => oterm CLambda [bterm [] (toSquiggle T); bterm [n] (toSquiggle b)]
+| tProd n T b => oterm CProd [bterm [] (toSquiggle T);  bterm [n] (toSquiggle b)]
+| tApp f args => oterm (CApply (length args)) (map ((bterm [])∘toSquiggle) (f::args))
+| _ => oterm CUnknown []
+end.
+
+
+Fixpoint fromSquiggle (t:@DTerm Ast.name CoqOpid) : term :=
+(* switch the side, remove toSquiggle from LHS, but fromSquiggle in RHS at the corresponding
+place *)
+match t with
+| vterm n => tRel (N.to_nat n)
+| oterm (CSort s) [] => tSort s
+| oterm CLambda [bterm [] T; bterm [n] b] =>  
+    tLambda n (fromSquiggle T) (fromSquiggle b)
+| oterm CProd [bterm [] T; bterm [n] b] =>  
+    tProd n (fromSquiggle T) (fromSquiggle b)
+| oterm (CApply _) ((bterm [] f)::args) =>
+    tApp (fromSquiggle f) (map (fromSquiggle ∘ get_nt) args)
+| _ => tUnknown ""
+end.
+
+Require Import SquiggleEq.tactics.
+Require Import SquiggleEq.LibTactics.
+Require Import Psatz.
+
+Lemma fromSquiggleFromSquiggleInv t:
+  getOpid (toSquiggle t) <> Some CUnknown
+  -> fromSquiggle (toSquiggle t) = t.
+Proof using.
+  induction t; unfold getOpid; simpl; intros Hneq; sp.
+- f_equal. lia.
+- f_equal; try rewrite IHt1; try rewrite IHt2; try reflexivity. admit. admit.
+- f_equal; try rewrite IHt1; try rewrite IHt2; try reflexivity. admit. admit.
+- repeat rewrite map_map. unfold compose. simpl. 
+  f_equal;[ apply IHt| setoid_rewrite <- (map_id l) at 2; apply eq_maps;
+      intros].
+  (* term_ind is weak *) admit.  admit.
+Abort.
+
+(*
+Definition toSqNamed (t:term) : @NTerm NVar 
+*)
+
+
+ 
